Rearrange dependencies to prepare for DoTransferRPC()
A shard server also uses shard clerks to talk to other shard servers, so
needed to shuffle around some definitions to be able to refer to the
clerk_proof definitions in the shard server proof.

src/program_proof/memkv/memkv_shard_proof.v
@@ -2,103 +2,11 @@ From Perennial.program_proof Require Import proof_prelude.
 From Goose.github_com.mit_pdos.gokv Require Import memkv.
 From Perennial.goose_lang Require Import ffi.grove_ffi.
 From Perennial.program_proof.lockservice Require Import rpc.
-From Perennial.program_proof.memkv Require Export memkv_marshal_get_proof memkv_marshal_install_shard_proof common_proof.
+From Perennial.program_proof.memkv Require Export memkv_shard_definitions common_proof.
 
 Section memkv_shard_proof.
 
 Context `{!heapG Σ, rpcG Σ GetReplyC}.
-
-Axiom kvptsto : gname → u64 → list u8 → iProp Σ.
-
-Global Instance kvptst_tmlss γkv k v : Timeless (kvptsto γkv k v).
-Admitted.
-
-Definition uKV_GET := 2.
-Definition uKV_INS_SHARD := 3.
-
-Record memkv_shard_names := {
- rpc_gn : rpc_names ;
- kv_gn : gname
-}
-.
-
-Implicit Type γ : memkv_shard_names.
-
-Definition own_shard γkv sid (m:gmap u64 (list u8)) : iProp Σ :=
-  [∗ set] k ∈ (fin_to_set u64), ⌜shardOfC k ≠ sid⌝ ∨
-                                kvptsto γkv k (default [] (m !! k))
-.
-
-Definition own_MemKVShardServer (s:loc) γ : iProp Σ :=
-  ∃ (lastReply_ptr lastSeq_ptr peers_ptr:loc) (kvss_sl shardMap_sl:Slice.t)
-    (lastReplyM:gmap u64 GetReplyC) (lastReplyMV:gmap u64 goose_lang.val) (lastSeqM:gmap u64 u64) (nextCID:u64) (shardMapping:list bool) (kvs_ptrs:list loc),
-  "HlastReply" ∷ s ↦[MemKVShardServer.S :: "lastReply"] #lastReply_ptr ∗
-  "HlastReplyMap" ∷ map.is_map lastReply_ptr (lastReplyMV, #0) ∗ (* TODO: default *)
-  "%HlastReplyMVdom" ∷ ⌜dom (gset u64) lastReplyMV = dom (gset u64) lastSeqM⌝ ∗
-  "HlastReply_structs" ∷ ([∗ map] k ↦ v;rep ∈ lastReplyMV ; lastReplyM, (∃ val_sl q, ⌜v = (#rep.(GR_Err), (slice_val val_sl, #()))%V⌝ ∗ typed_slice.is_slice_small val_sl byteT q rep.(GR_Value))) ∗
-  "HlastSeq" ∷ s ↦[MemKVShardServer.S :: "lastSeq"] #lastSeq_ptr ∗
-  "HlastSeqMap" ∷ is_map lastSeq_ptr lastSeqM ∗
-  "HnextCID" ∷ s ↦[MemKVShardServer.S :: "nextCID"] #nextCID ∗
-  "HshardMap" ∷ s ↦[MemKVShardServer.S :: "shardMap"] (slice_val shardMap_sl) ∗
-  "HshardMap_sl" ∷ typed_slice.is_slice shardMap_sl boolT 1%Qp shardMapping ∗
-  "Hkvss" ∷ s ↦[MemKVShardServer.S :: "kvss"] (slice_val kvss_sl) ∗
-  "Hkvss_sl" ∷ slice.is_slice kvss_sl (mapT (slice.T byteT)) 1%Qp (fmap (λ x:loc, #x) kvs_ptrs) ∗
-  "Hpeers" ∷ s ↦[MemKVShardServer.S :: "peers"] #peers_ptr ∗
-  "Hrpc" ∷ RPCServer_own_ghost γ.(rpc_gn) lastSeqM lastReplyM ∗
-  "%HshardMapLength" ∷ ⌜length shardMapping = uNSHARD⌝ ∗
-  "%HkvssLength" ∷ ⌜length kvs_ptrs = uNSHARD⌝ ∗
-  "HownShards" ∷ ([∗ set] sid ∈ (fin_to_set u64),
-                  ⌜(shardMapping !! (int.nat sid)) ≠ Some true⌝ ∨
-                  (∃ (kvs_ptr:loc) (m:gmap u64 (list u8)) (mv:gmap u64 goose_lang.val),
-                      own_shard γ.(kv_gn) sid m ∗ (* own shard *)
-                      ⌜kvs_ptrs !! (int.nat sid) = Some kvs_ptr⌝ ∗
-                      map.is_map kvs_ptr (mv, (slice_val Slice.nil)) ∗
-                      ([∗ set] k ∈ (fin_to_set u64),
-                       ⌜shardOfC k ≠ sid⌝ ∨ (∃ vsl, ⌜default (slice_val Slice.nil) (mv !! k) = (slice_val vsl)⌝ ∗ typed_slice.is_slice vsl byteT (1%Qp) (default [] (m !! k))) )
-                  )
-                 )
-.
-
-Definition memKVN := nroot .@ "memkv".
-
-Definition is_MemKVShardServer (s:loc) γ : iProp Σ :=
-  ∃ mu,
-  "#His_srv" ∷ is_RPCServer γ.(rpc_gn) ∗
-  "#Hmu" ∷ readonly (s ↦[MemKVShardServer.S :: "mu"] mu) ∗
-  "#HmuInv" ∷ is_lock memKVN mu (own_MemKVShardServer s γ)
-.
-
-Definition PreShardGet Eo Ei γ key Q : iProp Σ :=
-  |={Eo,Ei}=> (∃ v, kvptsto γ.(kv_gn) key v ∗ (kvptsto γ.(kv_gn) key v ={Ei,Eo}=∗ Q v))
-.
-
-Definition PostShardGet Eo Ei γ (key:u64) Q (rep:GetReplyC) : iProp Σ := ⌜rep.(GR_Err) ≠ 0⌝ ∗ (PreShardGet Eo Ei γ key Q) ∨
-                                                        ⌜rep.(GR_Err) = 0⌝ ∗ (Q rep.(GR_Value)).
-
-Definition is_shard_server host γ : iProp Σ :=
-  "#His_rpc" ∷ is_RPCServer γ.(rpc_gn) ∗
-  "#HgetSpec" ∷ handler_is (coPset * coPset * (list u8 → iProp Σ) * rpc_request_names) host uKV_GET
-             (λ x reqData, ∃ req, ⌜has_encoding_GetRequest reqData req⌝ ∗
-                                   is_RPCRequest γ.(rpc_gn) x.2 (PreShardGet x.1.1.1 x.1.1.2 γ req.(GR_Key) x.1.2)
-                                                            (PostShardGet x.1.1.1 x.1.1.2 γ req.(GR_Key) x.1.2)
-                                                            {| Req_CID:=req.(GR_CID); Req_Seq:=req.(GR_Seq) |}
-             ) (* pre *)
-             (λ x reqData repData, ∃ req rep, ⌜has_encoding_GetReply repData rep⌝ ∗
-                                              ⌜has_encoding_GetRequest reqData req⌝ ∗
-                                              (RPCRequestStale γ.(rpc_gn) {| Req_CID:=req.(GR_CID); Req_Seq:=req.(GR_Seq) |} ∨
-                                              RPCReplyReceipt γ.(rpc_gn) {| Req_CID:=req.(GR_CID); Req_Seq:=req.(GR_Seq) |} rep)
-             ) (* post *) ∗
-
-  "#HinstallSpec" ∷ handler_is (rpc_request_names) host uKV_INS_SHARD
-             (λ x reqData, ∃ args, ⌜has_encoding_InstallShardRequest reqData args⌝ ∗
-                                  ⌜int.nat args.(IR_Sid) < uNSHARD⌝ ∗
-                                  is_RPCRequest γ.(rpc_gn) x (own_shard γ.(kv_gn) args.(IR_Sid) args.(IR_Kvs))
-                                                            (λ _, True)
-                                                            {| Req_CID:=args.(IR_CID); Req_Seq:=args.(IR_Seq) |}
-             ) (* pre *)
-             (λ x reqData repData, True
-             ) (* post *)
-.
 
 Lemma wp_shardOf key :
   {{{
@@ -117,7 +25,7 @@ Qed.
 
 Lemma own_shard_agree key v γkv sid m:
   shardOfC key = sid →
-  own_shard γkv sid m -∗ kvptsto γkv key v -∗
+  own_shard (Σ:=Σ) γkv sid m -∗ kvptsto γkv key v -∗
   ⌜v = default [] (m !! key)⌝
 .
 Proof.
@@ -266,7 +174,7 @@ Proof.
         iFrame "#∗".
         iNext.
         iExists _,_,_, _, _, _, _, _.
-        iExists _, _, _.
+        iExists _, _, _, _.
         iFrame.
         done.
       }
@@ -298,7 +206,7 @@ Proof.
         iFrame "#∗".
         iNext.
         iExists _,_,_, _, _, _, _, _.
-        iExists _, _, _.
+        iExists _, _, _, _.
         iFrame.
         done.
       }
@@ -494,7 +402,7 @@ Proof.
         iFrame "HmuInv Hlocked".
         iNext.
         iExists _,_,_, _, _, _, _, _.
-        iExists _, _, _.
+        iExists _, _, _, _.
         iFrame.
         iSplitL "".
         {
@@ -582,7 +490,7 @@ Proof.
         iFrame "HmuInv Hlocked".
         iNext.
         iExists _,_,_, _, _, _, _, _.
-        iExists _, _, _.
+        iExists _, _, _, _.
         iFrame.
         iSplitL "".
         { iPureIntro.
