src/program_proof/memkv/shard_encoding_proof.v
@@ -1,4 +1,0 @@
-From Perennial.program_proof Require Import proof_prelude.
-From Goose.github_com.mit_pdos.gokv Require Import memkv.
-From Perennial.goose_lang Require Import ffi.grove_ffi.
-From Perennial.program_proof.lockservice Require Import rpc.
